heap_lang/lib/counter.v
@@ -1,4 +1,5 @@
 From iris.program_logic Require Export weakestpre.
+From iris.base_logic.lib Require Export invariants.
 From iris.heap_lang Require Export lang.
 From iris.proofmode Require Import tactics.
 From iris.algebra Require Import frac auth.
