heap_lang/lib/lock.v
@@ -1,4 +1,5 @@
-From iris.heap_lang Require Import heap notation.
+From iris.heap_lang Require Export rules notation.
+From iris.base_logic.lib Require Export invariants.
 
 Structure lock Σ `{!heapG Σ} := Lock {
   (* -- operations -- *)
