heap_lang/proofmode.v
@@ -1,7 +1,7 @@
 From iris.program_logic Require Export weakestpre.
 From iris.proofmode Require Import coq_tactics.
 From iris.proofmode Require Export tactics.
-From iris.heap_lang Require Export wp_tactics heap.
+From iris.heap_lang Require Export wp_tactics rules.
 Import uPred.
 
 Ltac wp_strip_later ::= iNext.
